Use consistent naming (#169)

theories/Core/Completeness/LogicalRelation/Definitions.v
@@ -3,8 +3,8 @@ From Mcltt Require Import Base.
 From Mcltt.Core Require Export PER.
 Import Domain_Notations.
 
-Inductive rel_exp M p M' p' (R : relation domain) : Prop :=
-| mk_rel_exp : forall m m', {{ ⟦ M ⟧ p ↘ m }} -> {{ ⟦ M' ⟧ p' ↘ m' }} -> {{ Dom m ≈ m' ∈ R }} -> rel_exp M p M' p' R.
+Inductive rel_exp M ρ M' ρ' (R : relation domain) : Prop :=
+| mk_rel_exp : forall m m', {{ ⟦ M ⟧ ρ ↘ m }} -> {{ ⟦ M' ⟧ ρ' ↘ m' }} -> {{ Dom m ≈ m' ∈ R }} -> rel_exp M ρ M' ρ' R.
 #[global]
 Arguments mk_rel_exp {_ _ _ _ _}.
 #[export]
@@ -12,9 +12,9 @@ Hint Constructors rel_exp : mcltt.
 
 Definition rel_exp_under_ctx Γ A M M' :=
   exists env_rel (_ : {{ EF Γ ≈ Γ ∈ per_ctx_env ↘ env_rel }}) i,
-  forall p p' (equiv_p_p' : {{ Dom p ≈ p' ∈ env_rel }}),
+  forall ρ ρ' (equiv_ρ_ρ' : {{ Dom ρ ≈ ρ' ∈ env_rel }}),
   exists (elem_rel : relation domain),
-     rel_typ i A p A p' elem_rel /\ rel_exp M p M' p' elem_rel.
+     rel_typ i A ρ A ρ' elem_rel /\ rel_exp M ρ M' ρ' elem_rel.
 
 Definition valid_exp_under_ctx Γ A M := rel_exp_under_ctx Γ A M M.
 #[global]
@@ -24,8 +24,8 @@ Hint Transparent valid_exp_under_ctx : mcltt.
 #[export]
 Hint Unfold valid_exp_under_ctx : mcltt.
 
-Inductive rel_sub σ p σ' p' (R : relation env) : Prop :=
-| mk_rel_sub : forall o o', {{ ⟦ σ ⟧s p ↘ o }} -> {{ ⟦ σ' ⟧s p' ↘ o' }} -> {{ Dom o ≈ o' ∈ R }} -> rel_sub σ p σ' p' R.
+Inductive rel_sub σ ρ σ' ρ' (R : relation env) : Prop :=
+| mk_rel_sub : forall ρσ ρ'σ', {{ ⟦ σ ⟧s ρ ↘ ρσ }} -> {{ ⟦ σ' ⟧s ρ' ↘ ρ'σ' }} -> {{ Dom ρσ ≈ ρ'σ' ∈ R }} -> rel_sub σ ρ σ' ρ' R.
 #[global]
 Arguments mk_rel_sub {_ _ _ _ _ _}.
 #[export]
@@ -34,8 +34,8 @@ Hint Constructors rel_sub : mcltt.
 Definition rel_sub_under_ctx Γ Δ σ σ' :=
   exists env_rel (_ : {{ EF Γ ≈ Γ ∈ per_ctx_env ↘ env_rel }})
      env_rel' (_ : {{ EF Δ ≈ Δ ∈ per_ctx_env ↘ env_rel' }}),
-  forall p p' (equiv_p_p' : {{ Dom p ≈ p' ∈ env_rel }}),
-    rel_sub σ p σ' p' env_rel'.
+  forall ρ ρ' (equiv_ρ_ρ' : {{ Dom ρ ≈ ρ' ∈ env_rel }}),
+    rel_sub σ ρ σ' ρ' env_rel'.
 
 Definition valid_sub_under_ctx Γ Δ σ := rel_sub_under_ctx Γ Δ σ σ.
 #[global]
@@ -47,8 +47,8 @@ Hint Unfold valid_sub_under_ctx : mcltt.
 
 Definition subtyp_under_ctx Γ M M' :=
   exists env_rel (_ : {{ EF Γ ≈ Γ ∈ per_ctx_env ↘ env_rel }}) i,
-  forall p p' (equiv_p_p' : {{ Dom p ≈ p' ∈ env_rel }}),
-    exists R R', rel_typ i M p M p' R /\ rel_typ i M' p M' p' R' /\ rel_exp M p M' p' (per_subtyp i).
+  forall ρ ρ' (equiv_ρ_ρ' : {{ Dom ρ ≈ ρ' ∈ env_rel }}),
+    exists R R', rel_typ i M ρ M ρ' R /\ rel_typ i M' ρ M' ρ' R' /\ rel_exp M ρ M' ρ' (per_subtyp i).
 
 Notation "⊨ Γ ≈ Γ'" := (per_ctx Γ Γ')  (in custom judg at level 80, Γ custom exp, Γ' custom exp).
 Notation "⊨ Γ" := (valid_ctx Γ) (in custom judg at level 80, Γ custom exp).
