theories/Core/Semantic/NbE.v
@@ -7,18 +7,18 @@ Generalizable All Variables.
 Inductive initial_env : ctx -> env -> Prop :=
 | initial_env_nil : initial_env nil empty_env
 | initial_env_cons :
-  `( initial_env Γ p ->
-     {{ ⟦ A ⟧ p ↘ a }} ->
-     initial_env (A :: Γ) d{{{ p ↦ ⇑! a (length Γ) }}}).
+  `( initial_env Γ ρ ->
+     {{ ⟦ A ⟧ ρ ↘ a }} ->
+     initial_env (A :: Γ) d{{{ ρ ↦ ⇑! a (length Γ) }}}).
 
 #[export]
 Hint Constructors initial_env : mcltt.
 
-Lemma functional_initial_env : forall Γ p,
-    initial_env Γ p ->
-    forall p',
-      initial_env Γ p' ->
-      p = p'.
+Lemma functional_initial_env : forall Γ ρ,
+    initial_env Γ ρ ->
+    forall ρ',
+      initial_env Γ ρ' ->
+      ρ = ρ'.
 Proof.
   induction 1; intros ? Hother; inversion_clear Hother; eauto.
   erewrite IHinitial_env in *; try eassumption;
@@ -32,16 +32,16 @@ Hint Resolve functional_initial_env : mcltt.
 Ltac functional_initial_env_rewrite_clear1 :=
   let tactic_error o1 o2 := fail 3 "functional_initial_env equality between" o1 "and" o2 "cannot be solved by mauto" in
   match goal with
-  | H1 : initial_env ?G ?p, H2 : initial_env ?G ?p' |- _ =>
-      clean replace p' with p by first [solve [mauto 2] | tactic_error p' p]; clear H2
+  | H1 : initial_env ?G ?ρ, H2 : initial_env ?G ?ρ' |- _ =>
+      clean replace ρ' with ρ by first [solve [mauto 2] | tactic_error ρ' ρ]; clear H2
   end.
 Ltac functional_initial_env_rewrite_clear := repeat functional_initial_env_rewrite_clear1.
 
 Inductive nbe : ctx -> exp -> typ -> nf -> Prop :=
 | nbe_run :
-  `( initial_env Γ p ->
-     {{ ⟦ A ⟧ p ↘ a }} ->
-     {{ ⟦ M ⟧ p ↘ m }} ->
+  `( initial_env Γ ρ ->
+     {{ ⟦ A ⟧ ρ ↘ a }} ->
+     {{ ⟦ M ⟧ ρ ↘ m }} ->
      {{ Rnf ⇓ a m in (length Γ) ↘ w }} ->
      nbe Γ M A w ).
 
@@ -117,8 +117,8 @@ Hint Resolve functional_nbe_of_typ : mcltt.
 
 Inductive nbe_ty : ctx -> typ -> nf -> Prop :=
 | nbe_ty_run :
-  `( initial_env Γ p ->
-     {{ ⟦ M ⟧ p ↘ m }} ->
+  `( initial_env Γ ρ ->
+     {{ ⟦ M ⟧ ρ ↘ m }} ->
      {{ Rtyp m in (length Γ) ↘ W }} ->
      nbe_ty Γ M W ).
 
